Lean4/Test.lean
@@ -1,0 +1,7 @@
+import Mathlib.Data.Nat.Basic
+
+theorem rangeDecompose (start mid stop : ℕ) (hs : start ≤ mid ∧ mid ≤ stop)
+  {f : ℕ → β → Id (ForInStep β)} :
+  STD.forIn (mkRange' start stop) init f =
+    STD.forIn (mkRange' mid stop) (Id.run (STD.forIn (mkRange' start mid) init f)) f := by
+  sorry
